added proofs in Feedback_MW.thy, InnerProd_Case_Study.thy and SPF_MW.thy

Feedback_MW.thy
@@ -1,5 +1,5 @@
 theory Feedback_MW
-imports SPF SBTheorie ParComp_MW StreamCase_Study
+imports SPF Streams SBTheorie ParComp_MW StreamCase_Study SPF_MW SerComp_JB
 
 begin
 
@@ -59,11 +59,17 @@ lemma spfadd_cont[simp]: "cont (\<lambda> sb. (sbDom\<cdot>sb = {ch1, ch2})
 definition delay:: "nat stream  \<rightarrow> nat stream" where
 "delay \<equiv> \<Lambda> s . \<up>0 \<bullet> s"
 
-lemma spfdelay_mono[simp] : "monofun 
-                           (\<lambda> i. (\<lambda> sb. (sbDom\<cdot>sb = {ch3}) \<leadsto> ([ch2\<mapsto>delay\<cdot>((Y i) . ch3)]\<Omega>)))"
-sorry
+lemma spfdelay_mono[simp] : "monofun (\<lambda> sb. (sbDom\<cdot>sb = {ch3}) \<leadsto> ([ch2\<mapsto>delay\<cdot>(sb . ch3)]\<Omega>))"
+  apply (rule spf_mono2monofun)
+   apply (rule spf_monoI)
+   apply (simp add: domIff2)
+   apply (rule sb_below)
+    apply (simp add: sbdom_insert)
+    apply (simp add: sbdom_rep_eq sbgetch_rep_eq)
+   apply (meson monofun_cfun monofun_cfun_arg monofun_cfun_fun)
+   by (rule, simp add: domIff2)
 
-lemma delay_chain[simp]: "chain Y \<Longrightarrow> sbDom\<cdot>(Y 0) = {ch1,ch2} 
+lemma delay_chain[simp]: "chain Y \<Longrightarrow> sbDom\<cdot>(Y 0) = {ch3} 
                         \<Longrightarrow> chain (\<lambda> i. [ch2\<mapsto>delay\<cdot>((Y i) . ch3)]\<Omega>)"
   apply (rule chainI)
   apply (rule sb_below)
@@ -71,21 +77,35 @@ lemma delay_chain[simp]: "chain Y \<Longrightarrow> sbDom\<cdot>(Y 0) = {ch1,ch2
    apply (simp add: sbdom_rep_eq sbgetch_rep_eq)
    by (simp add: monofun_cfun po_class.chainE)
 
-lemma delay_chain_lub[simp]: "chain Y \<Longrightarrow> sbDom\<cdot>(Lub Y) = {ch1,ch2} 
+lemma delay_chain_lub[simp]: "chain Y \<Longrightarrow> sbDom\<cdot>(Lub Y) = {ch3} 
                                 \<Longrightarrow> chain (\<lambda> i. [ch2\<mapsto>delay\<cdot>((Y i) . ch3)]\<Omega>)"
   by (simp add: sbChain_dom_eq2)
 
-lemma sdelay_Lub[simp]: "chain Y \<Longrightarrow> sbDom\<cdot>(Lub Y) = {ch1,ch2} \<Longrightarrow> 
-  (\<Squnion>i. add\<cdot>(Y i . ch1)\<cdot>(Y i . ch2)) = add\<cdot>((Lub Y) . ch1)\<cdot>((Lub Y). ch2)"
-sorry
+lemma delay_Lub[simp]: "chain Y \<Longrightarrow> sbDom\<cdot>(Lub Y) = {ch3} \<Longrightarrow> 
+  (\<Squnion>i. delay\<cdot>(Y i . ch3)) = delay\<cdot>((Lub Y). ch3)"
+  by (simp add: lub_distribs(1) lub_eval)
 
 lemma spfdelay_chain [simp]: "chain Y \<Longrightarrow>
-      chain (\<lambda> i. (\<lambda> sb. (sbDom\<cdot>sb = {ch3}) \<leadsto> ([ch2\<mapsto>delay\<cdot>((Y i) . ch3)]\<Omega>)))"
-sorry
+      chain (\<lambda> i. (sbDom\<cdot>(Y i) = {ch3}) \<leadsto> ([ch2\<mapsto>delay\<cdot>((Y i) . ch3)]\<Omega>))"
+  apply (rule chainI)
+  apply (simp add: sbChain_dom_eq2)
+  apply (rule impI, rule some_below, rule sb_below)
+   apply (simp add: sbdom_rep_eq)
+  apply (simp add: sbdom_rep_eq sbgetch_rep_eq)
+  by (simp add: monofun_cfun po_class.chainE)
 
 lemma spfdelay_cont[simp]: "cont (\<lambda> sb. (sbDom\<cdot>sb = {ch3}) 
                                 \<leadsto> ([ch2\<mapsto>delay\<cdot>(sb . ch3)]\<Omega>))" (is "cont ?F")
-sorry
+  apply (rule spf_cont2cont)
+    apply (rule spf_contlubI)
+    apply (simp add: domIff2 sbChain_dom_eq2)
+    apply (rule sb_below)
+     apply (simp add: sbdom_rep_eq )
+     apply (simp only: Cfun.contlub_cfun_arg delay_chain_lub)
+     apply (simp add: sbdom_rep_eq sbgetch_rep_eq)
+    apply (simp add: sbdom_rep_eq sbgetch_rep_eq sbgetch_lub)
+   apply (simp add: monofun2spf_mono)
+  by(simp add: domIff2, rule+)
 
 
 (* SPF Definition *)
@@ -139,9 +159,26 @@ lemma [simp]: "Oc addC delayC = {c2, c3}"
 lemma [simp]: "I addC delayC = {c1}"
 by(auto simp add: I_def)
 
+lemma [simp]: "spfDom\<cdot>(spfcomp addC delayC) = {c1}"
+by(simp add: spfComp_dom_I)
+
+lemma [simp]: "spfRan\<cdot>(spfcomp addC delayC) = {c2, c3}"
+by(simp add: spfComp_ran_Oc)
+
+(* prerequirements for final lemma *)
+
 (* final lemma *)
 
+definition sum1 :: "nat SPF" where
+"sum1 \<equiv> hide (addC \<otimes>  delayC) {c2}"
 
+lemma sum1EqCh: assumes "sbDom\<cdot>sb = I addC delayC" shows "(sum1 \<rightleftharpoons> sb) . c3 = ((addC \<otimes>  delayC) \<rightleftharpoons> sb) . c3"
+apply(simp add: sum1_def)
+apply(subst hideSbRestrictCh)
+by(simp_all add: assms)
 
+lemma sumEq: assumes "sbDom\<cdot>sb = I addC delayC" shows "(sum1 \<rightleftharpoons> sb) . c3 = sum4\<cdot>(sb . c1)"
+apply(subst sum1EqCh, simp add: assms)
+sorry
 
 end
